scratch/Scratch_FibMem.thy
@@ -1,0 +1,76 @@
+theory Scratch_FibMem
+  imports Refine_Imperative_HOL.IICF "dp/Monad"
+begin
+
+fun fib :: "nat \<Rightarrow> int" where
+  "fib 0 = 1"
+| "fib (Suc 0) = 1"
+| "fib (Suc (Suc n)) = fib (Suc n) + fib n"
+
+type_synonym tab = "int list"
+
+(*Since fib n \<ge> 0, negative value is used here to represent None*)
+definition is_some :: "int \<Rightarrow> bool" where
+  "is_some v \<equiv> v \<ge> 0"
+
+definition checkmem :: "tab \<Rightarrow> nat \<Rightarrow> (tab \<times> int) nres \<Rightarrow> (tab \<times> int) nres" where
+  "checkmem M n v \<equiv> do {
+    fn \<leftarrow> mop_list_get M n;
+    if is_some fn
+      then RETURN (M, fn)
+      else do {
+        (M, fn) \<leftarrow> v;
+        M \<leftarrow> mop_list_set M n fn;
+        RETURN (M, fn)
+      }
+    }"
+
+definition fib_rec_mem_body :: "((tab \<times> nat) \<Rightarrow> (tab \<times> int) nres) \<Rightarrow> (tab \<times> nat) \<Rightarrow> (tab \<times> int) nres" where
+  "fib_rec_mem_body \<equiv> \<lambda>f (M, n). checkmem M n (do {
+    if n < 2
+      then RETURN (M, 1)
+      else do {
+        (M, f0) \<leftarrow> f (M, n-2);
+        (M, f1) \<leftarrow> f (M, n-1);
+        RETURN (M, f0 + f1)
+      }
+    })"
+
+definition fib_rec_mem :: "nat \<Rightarrow> int nres" where
+  "fib_rec_mem n \<equiv> do {
+    (_, v) \<leftarrow> RECT fib_rec_mem_body (replicate (n+1) (-1), n);
+    RETURN v
+   }"
+
+sepref_definition fib_rec_mem1 is fib_rec_mem :: "nat_assn\<^sup>k \<rightarrow>\<^sub>a int_assn"
+  unfolding fib_rec_mem_def fib_rec_mem_body_def checkmem_def is_some_def
+  apply (rewrite in "RECT _ (\<hole>, _)" array_fold_custom_of_list)
+  by sepref
+
+definition fib_rec_mem_body' where
+  "fib_rec_mem_body' \<equiv> \<lambda>f n. "
+
+term 0 (*
+
+definition cmem :: "tab \<Rightarrow> bool" where
+  "cmem M \<equiv> \<forall>i. i<length M \<longrightarrow> M!i\<ge>0 \<longrightarrow> M!i=fib i"
+
+lemma cmem_intro:
+  assumes "\<And>i. i<length M \<Longrightarrow> M!i\<ge>0 \<Longrightarrow> M!i=fib i"
+  shows "cmem M"
+  using assms unfolding cmem_def by fastforce
+
+lemma cmem_elim:
+  assumes "cmem M" "i < length M"
+  obtains "M!i < 0" | "fib i = M!i "
+  using assms unfolding cmem_def by fastforce
+  term 0 
+
+lemma cmem_update:
+  "\<lbrakk>cmem M; v = fib i\<rbrakk> \<Longrightarrow> cmem (list_update M i v)"
+  by (fastforce intro!: cmem_intro elim: cmem_elim simp: nth_list_update')
+
+definition crel_vs :: "'a nres \<Rightarrow> (tab \<times> 'a) nres \<Rightarrow> bool" where
+  "crel_vs v s \<equiv> nofail v \<longrightarrow> the"
+
+end
