scratch/dp/DP_CPredS.thy
@@ -1,0 +1,54 @@
+theory DP_CPredS
+  imports "./DP_CRelVS"
+begin
+locale dp_pred =
+  fixes cmem :: "('param \<rightharpoonup> 'result) \<Rightarrow> bool"
+begin
+context 
+  includes lifting_syntax
+begin
+  
+definition cpred_s :: "('a \<Rightarrow> bool) \<Rightarrow> ('param \<rightharpoonup> 'result, 'a) state \<Rightarrow> bool" where
+  "cpred_s P s \<equiv> \<forall>M. cmem M \<longrightarrow> (case runState s M of (v', M') \<Rightarrow> P v' \<and> cmem M')"
+  
+lemma cpred_s_def_alt: "cpred_s P s = pred_fun cmem (pred_prod P cmem) (runState s)"
+  unfolding cpred_s_def by (fastforce split: pred_prod_split)
+term 0(**)
+
+notation pred_fun (infixr "...>" 55)
+
+abbreviation pred_fun_lifted :: "('a \<Rightarrow> bool) \<Rightarrow> ('b \<Rightarrow> bool) \<Rightarrow> ('a ==_\<Longrightarrow> 'b) \<Rightarrow> bool" (infixr "...>\<^sub>T" 55) where
+  "A ...>\<^sub>T B \<equiv> A ...> cpred_s B"
+
+  
+lemma cpred_s_intro:
+  assumes "\<And>M v' M'. \<lbrakk>cmem M; runState v\<^sub>T M = (v', M')\<rbrakk> \<Longrightarrow> P v' \<and> cmem M'"
+  shows "cpred_s P v\<^sub>T"
+  unfolding cpred_s_def using assms by blast
+
+lemma cpred_s_elim:
+  assumes "cpred_s P v\<^sub>T" "cmem M"
+  obtains v' M' where "runState v\<^sub>T M = (v', M')" "P v'" "cmem M'"
+  using assms unfolding cpred_s_def by blast
+term 0 (**)
+
+lemma cpred_s_return:
+  "P v \<Longrightarrow> cpred_s P \<langle>v\<rangle>"
+  unfolding return_def by (fastforce intro: cpred_s_intro)
+
+lemma return_transferP:
+  "(P ...> cpred_s P) return"
+  unfolding pred_fun_def by (metis cpred_s_return)
+    
+lemma bind_transferP:
+  "(cpred_s P0 ...> (P0 ...>\<^sub>T P1) ...> cpred_s P1) (op \<bind>)"
+  unfolding bind_def pred_fun_def by (fastforce intro: cpred_s_intro elim: cpred_s_elim split: prod.split)
+    
+lemma fun_app_lifted_transferP:
+  "(cpred_s (R0 ...>\<^sub>T R1) ...> cpred_s P0 ...> cpred_s P1) (op .)"
+  unfolding fun_app_lifted_def
+  oops 
+end
+end
+
+end
