scratch/dp/DP_CRelVS.thy
@@ -1,0 +1,374 @@
+theory DP_CRelVS
+  imports "./Monad" "./DP_Lifting"
+begin
+  
+definition rel_imp :: "('a \<Rightarrow> 'b \<Rightarrow> bool) \<Rightarrow> ('a \<Rightarrow> 'b \<Rightarrow> bool) \<Rightarrow> bool" where
+  "rel_imp R R' \<equiv> \<forall>x y. R x y \<longrightarrow> R' x y"
+term 0 (**)
+
+locale dp_consistency =
+  fixes dp :: "'param \<Rightarrow> 'result"
+begin
+  
+context
+  includes lifting_syntax
+begin
+  
+  (* Predicates *)
+definition cmem :: "('param \<rightharpoonup> 'result) \<Rightarrow> bool" where
+  "cmem M \<equiv> \<forall>param\<in>dom M. M param = Some (dp param)"
+term 0 (**)
+  
+definition crel_vs :: "('a \<Rightarrow> 'b \<Rightarrow> bool) \<Rightarrow> 'a \<Rightarrow> ('param \<rightharpoonup> 'result, 'b) state \<Rightarrow> bool" where
+  "crel_vs R v s \<equiv> \<forall>M. cmem M \<longrightarrow> (case runState s M of (v', M') \<Rightarrow> R v v' \<and> cmem M')"
+  
+definition crel_vs_alt :: "('a \<Rightarrow> 'b \<Rightarrow> bool) \<Rightarrow> 'a \<Rightarrow> ('param \<rightharpoonup> 'result, 'b) state \<Rightarrow> bool" where
+  "crel_vs_alt R v s \<equiv> pred_fun cmem (pred_prod (R v) cmem) (runState s)"
+
+abbreviation rel_fun_lifted :: "('a \<Rightarrow> 'c \<Rightarrow> bool) \<Rightarrow> ('b \<Rightarrow> 'd \<Rightarrow> bool) \<Rightarrow> ('a \<Rightarrow> 'b) \<Rightarrow> ('c ==_\<Longrightarrow> 'd) \<Rightarrow> bool" (infixr "===>\<^sub>T" 55) where
+  "rel_fun_lifted R R' \<equiv> R ===> crel_vs R'"
+term 0 (**)
+
+lemma "crel_vs = crel_vs_alt"
+  unfolding crel_vs_def crel_vs_alt_def
+  by (fastforce split: pred_prod_split)
+
+definition consistentDP :: "('param \<Rightarrow>\<^sub>T 'result) \<Rightarrow> bool" where
+  "consistentDP \<equiv> (op = ===> crel_vs op =) dp"
+term 0 (**)
+  
+  (* cmem *)
+lemma cmem_intro:
+  assumes "\<And>param v. M param = Some v \<Longrightarrow> v = dp param"
+  shows "cmem M"
+  using assms unfolding cmem_def by blast
+term 0 (**)
+  
+lemma cmem_elim:
+  assumes "cmem M" "M param = Some v"
+  obtains "dp param = v"
+  using assms unfolding cmem_def dom_def by auto
+term 0 (**)
+  
+  (* crel_vs *)
+lemma crel_vs_intro:
+  assumes "\<And>M v' M'. \<lbrakk>cmem M; runState v\<^sub>T M = (v', M')\<rbrakk> \<Longrightarrow> R v v' \<and> cmem M'"
+  shows "crel_vs R v v\<^sub>T"
+  using assms unfolding crel_vs_def by blast
+term 0 (**)
+  
+lemma crel_vs_elim:
+  assumes "crel_vs R v v\<^sub>T" "cmem M"
+  obtains v' M' where "runState v\<^sub>T M = (v', M')" "R v v'" "cmem M'"
+  using assms unfolding crel_vs_def by blast
+term 0 (**)
+  
+lemma crel_vs_mono:
+  assumes "crel_vs R v s" "rel_imp R R'"
+  shows "crel_vs R' v s"
+  using assms unfolding rel_imp_def by (fastforce intro: crel_vs_intro elim: crel_vs_elim)
+
+  (* consistentDP *)
+lemma consistentDP_intro:
+  assumes "\<And>param. crel_vs (op =) (dp param) (dp\<^sub>T param)"
+  shows "consistentDP dp\<^sub>T"
+  using assms unfolding consistentDP_def by blast
+term 0 (**)
+  
+lemma crel_vs_return:
+  "\<lbrakk>R x y\<rbrakk> \<Longrightarrow> crel_vs R x (return y)"
+  unfolding return_def by (fastforce intro: crel_vs_intro)
+term 0 (**)
+  
+  (* Low level operators *)
+lemma cmem_upd:
+  "\<lbrakk>cmem M; v = dp param\<rbrakk> \<Longrightarrow> cmem (M(param\<mapsto>v))"
+  unfolding cmem_def by auto
+term 0 (**)
+  
+lemma crel_vs_get:
+  "\<lbrakk>\<And>M. cmem M \<Longrightarrow> crel_vs R v (sf M)\<rbrakk> \<Longrightarrow> crel_vs R v (get \<bind> sf)"
+  unfolding get_def bind_def by (fastforce intro: crel_vs_intro elim: crel_vs_elim split: prod.split)
+term 0 (**)
+  
+lemma crel_vs_put:
+  "\<lbrakk>crel_vs R v sf; cmem M\<rbrakk> \<Longrightarrow> crel_vs R v (put M \<then> sf)"
+  unfolding put_def bind_def by (fastforce intro: crel_vs_intro elim: crel_vs_elim split: prod.split)
+term 0 (**)
+  
+lemma crel_vs_bind_eq:
+  "\<lbrakk>crel_vs op = v s; crel_vs R (f v) (sf v)\<rbrakk> \<Longrightarrow> crel_vs R (f v) (s \<bind> sf)"
+  unfolding bind_def rel_fun_def by (fastforce intro: crel_vs_intro elim: crel_vs_elim split: prod.split)
+term 0 (**)
+  
+lemma crel_vs_checkmem:
+  "\<lbrakk>crel_vs op = (dp param) s\<rbrakk> \<Longrightarrow> crel_vs op = (dp param) (checkmem param s)"
+  unfolding checkmem_def by (fastforce intro: crel_vs_return crel_vs_get crel_vs_put
+      crel_vs_bind_eq cmem_upd elim: cmem_elim split: option.splits)
+term 0 (**)
+  
+  (** Transfer rules **)
+  (* Basics *)
+lemma return_transfer[transfer_rule]:
+  "(R ===>\<^sub>T R) (\<lambda>x. x) return"
+  unfolding id_def rel_fun_def by (metis crel_vs_return)
+    
+lemma bind_transfer[transfer_rule]:
+  "(crel_vs R0 ===> (R0 ===>\<^sub>T R1) ===> crel_vs R1) (\<lambda>v f. f v) (op \<bind>)"
+  unfolding bind_def rel_fun_def by (fastforce intro: crel_vs_intro elim: crel_vs_elim split: prod.split)
+    
+lemma fun_app_lifted_transfer[transfer_rule]:
+  "(crel_vs (R0 ===>\<^sub>T R1) ===> crel_vs R0 ===> crel_vs R1) (\<lambda> f x. f x) (op .)"
+  unfolding fun_app_lifted_def by transfer_prover
+    
+lemma crel_vs_fun_app:
+  "\<lbrakk>crel_vs (R0 ===>\<^sub>T R1) f f\<^sub>T; crel_vs R0 x x\<^sub>T\<rbrakk> \<Longrightarrow> crel_vs R1 (f x) (f\<^sub>T . x\<^sub>T)"
+  using fun_app_lifted_transfer[THEN rel_funD, THEN rel_funD] .
+    
+term 0 (**)
+
+lemma unlift_'_transfer[transfer_rule]:
+  "(R ===> crel_vs R) (\<lambda> x. x) unlift_'"
+  unfolding unlift_'_def by transfer_prover
+term 0 (**)
+  
+lemma unlift_3_transfer[transfer_rule]:
+  "((R0 ===>\<^sub>T R1) ===> (R0 ===> crel_vs R1)) (\<lambda> f x. f x) unlift_3"
+  unfolding unlift_3_def by transfer_prover
+term 0 (**)
+  
+lemma unlift_33_transfer[transfer_rule]:
+  "((R0 ===>\<^sub>T R1 ===>\<^sub>T R2) ===> (R0 ===> R1 ===> crel_vs R2)) (\<lambda> f x0 x1. f x0 x1) unlift_33"
+  unfolding unlift_33_def by transfer_prover
+
+lemma lift_'_transfer[transfer_rule]:
+  "(R ===> crel_vs R) (\<lambda> x. x) lift_'"
+  unfolding lift_'_def by transfer_prover
+
+lemma lift_3_transfer[transfer_rule]:
+  "((R0 ===> R1) ===> crel_vs (R0 ===>\<^sub>T R1)) (\<lambda> f x. f x) lift_3"
+  unfolding lift_3_def by transfer_prover
+    
+lemma lift_33_transfer[transfer_rule]:
+  "((R0 ===> R1 ===> R2) ===> crel_vs (R0 ===>\<^sub>T R1 ===>\<^sub>T R2)) (\<lambda> f x0 x1. f x0 x1) lift_33"
+  unfolding lift_33_def by transfer_prover
+
+lemma lift_333_transfer[transfer_rule]:
+  "((R0 ===> R1 ===> R2 ===> R3) ===> crel_vs (R0 ===>\<^sub>T R1 ===>\<^sub>T R2 ===>\<^sub>T R3)) (\<lambda> f x0 x1 x2. f x0 x1 x2) lift_333"
+  unfolding lift_333_def by transfer_prover
+term 0 (**)
+
+  (* HOL *)
+lemma If_transfer[transfer_rule]:
+  "crel_vs (op = ===>\<^sub>T R ===>\<^sub>T R ===>\<^sub>T R) If If\<^sub>T"
+  unfolding If\<^sub>T_def by transfer_prover
+  
+lemma id_transfer[transfer_rule]:
+  "crel_vs (R ===>\<^sub>T R) id id\<^sub>T"
+  unfolding id_def id\<^sub>T_def by transfer_prover
+    
+lemma comp_transfer[transfer_rule]:
+  "crel_vs ((R1 ===>\<^sub>T R2) ===>\<^sub>T (R0 ===>\<^sub>T R1) ===>\<^sub>T (R0 ===>\<^sub>T R2)) comp comp\<^sub>T"
+  unfolding comp_def comp\<^sub>T_def fun_app_lifted_def by transfer_prover
+term 0 (**)
+
+  (* Arithmetic *)
+
+lemma plus_transfer[transfer_rule]:
+  "crel_vs (op = ===>\<^sub>T op = ===>\<^sub>T op =) plus plus\<^sub>T"
+  unfolding plus\<^sub>T_def by transfer_prover
+  
+lemma min_transfer[transfer_rule]:
+  "crel_vs (op = ===>\<^sub>T op = ===>\<^sub>T op =) min min\<^sub>T"
+  unfolding min\<^sub>T_def by transfer_prover
+    
+lemma max_transfer[transfer_rule]:
+  "crel_vs (op = ===>\<^sub>T op = ===>\<^sub>T op =) max max\<^sub>T"
+  unfolding max\<^sub>T_def by transfer_prover
+term 0 (**)  
+
+  (* Option *)
+lemma case_option_transfer[transfer_rule]:
+  "crel_vs (R1 ===>\<^sub>T (R0 ===>\<^sub>T R1) ===>\<^sub>T rel_option R0 ===>\<^sub>T R1) case_option case_option\<^sub>T"
+  unfolding case_option\<^sub>T_def by transfer_prover
+
+lemma None_transfer[transfer_rule]:
+  "crel_vs (rel_option R) None None\<^sub>T"
+  unfolding None\<^sub>T_def by transfer_prover
+
+lemma Some_transfer[transfer_rule]:
+  "crel_vs (R ===>\<^sub>T rel_option R) Some Some\<^sub>T"
+  unfolding Some\<^sub>T_def by transfer_prover
+term 0 (**)
+
+  (* List *)  
+lemma case_list_transfer[transfer_rule]:
+  "crel_vs (R1 ===>\<^sub>T (R0 ===>\<^sub>T list_all2 R0 ===>\<^sub>T R1) ===>\<^sub>T list_all2 R0 ===>\<^sub>T R1) case_list case_list\<^sub>T"
+  unfolding case_list\<^sub>T_def by transfer_prover
+  
+lemma Nil_transfer[transfer_rule]:
+  "crel_vs (list_all2 R) Nil Nil\<^sub>T"
+  unfolding Nil\<^sub>T_def by transfer_prover
+
+lemma Cons_transfer[transfer_rule]:
+  "crel_vs (R ===>\<^sub>T list_all2 R ===>\<^sub>T list_all2 R) Cons Cons\<^sub>T"
+  unfolding Cons\<^sub>T_def by transfer_prover
+    
+lemma upt_transfer[transfer_rule]:
+  "crel_vs (op = ===>\<^sub>T op = ===>\<^sub>T list_all2 op =) upt upt\<^sub>T"
+  unfolding upt\<^sub>T_def by transfer_prover
+term 0 (**)
+  
+  (* Prod *)
+lemma case_prod_transfer[transfer_rule]:
+  "crel_vs ((R0 ===>\<^sub>T R1 ===>\<^sub>T R2) ===>\<^sub>T rel_prod R0 R1 ===>\<^sub>T R2) case_prod case_prod\<^sub>T"
+  unfolding case_prod\<^sub>T_def by transfer_prover
+term 0 (**)
+  
+lemma Pair_transfer[transfer_rule]:
+  "crel_vs (R0 ===>\<^sub>T R1 ===>\<^sub>T rel_prod R0 R1) Pair Pair\<^sub>T"
+  unfolding Pair\<^sub>T_def by transfer_prover
+term 0 (**)
+
+  (* Combinator *)
+lemma map_transfer[transfer_rule]:
+  "crel_vs ((R0 ===>\<^sub>T R1) ===>\<^sub>T list_all2 R0 ===>\<^sub>T list_all2 R1) map map\<^sub>T"
+proof -
+  have [transfer_rule]: "((R0 ===>\<^sub>T R1) ===> (list_all2 R0 ===>\<^sub>T list_all2 R1)) map map\<^sub>T'"
+    apply ((rule rel_funI)+, induct_tac rule: list_all2_induct, assumption; unfold list.map map\<^sub>T'.simps)
+    subgoal premises [transfer_rule] by transfer_prover
+    subgoal premises [transfer_rule] by transfer_prover
+    done
+  show ?thesis
+    unfolding map\<^sub>T_def by transfer_prover
+qed
+  
+lemma fold_transfer[transfer_rule]:
+  "crel_vs ((R0 ===>\<^sub>T R1 ===>\<^sub>T R1) ===>\<^sub>T list_all2 R0 ===>\<^sub>T R1 ===>\<^sub>T R1) fold fold\<^sub>T"
+proof -
+  have [transfer_rule]: "((R0 ===>\<^sub>T R1 ===>\<^sub>T R1) ===> list_all2 R0 ===>\<^sub>T R1 ===>\<^sub>T R1) fold fold\<^sub>T'"
+    apply ((rule rel_funI)+, induct_tac rule: list_all2_induct, assumption; unfold fold.simps fold\<^sub>T'.simps)
+    subgoal premises [transfer_rule] by transfer_prover
+    subgoal premises [transfer_rule] by transfer_prover
+    done
+  show ?thesis
+    unfolding fold\<^sub>T_def by transfer_prover
+qed
+  
+definition "and_leftp R P x y \<equiv> R x y \<and> P x"
+
+lemma eq_onp_and_leftp_eq: "and_leftp (op =) P x y \<longleftrightarrow> eq_onp P x y"
+  unfolding and_leftp_def eq_onp_def by auto
+
+lemma and_leftp_elim: "and_leftp R P x y \<Longrightarrow> (R x y \<Longrightarrow> P x \<Longrightarrow> thesis) \<Longrightarrow> thesis"
+  unfolding and_leftp_def by auto
+term 0 (**)
+
+lemma and_leftp_leftset_intro:
+  "list_all2 R xs xs\<^sub>T' \<Longrightarrow> list_all2 (and_leftp R (\<lambda>x. x\<in>set xs)) xs xs\<^sub>T'"
+  unfolding list_all2_iff and_leftp_def set_zip by auto
+term 0 (**)
+  
+lemma and_leftp_lefteq_elim:
+  assumes "and_leftp R (op = y) x x\<^sub>T'"
+  obtains "x = y" "R y x\<^sub>T'"
+  using assms unfolding and_leftp_def by auto
+
+lemma and_leftp_lefteq_same:
+  "R x x\<^sub>T' \<Longrightarrow> and_leftp R (op = x) x x\<^sub>T'"
+  unfolding and_leftp_def by auto
+
+lemma and_leftp_crel_vs:
+  "and_leftp (crel_vs R) P x x\<^sub>T \<Longrightarrow> crel_vs (and_leftp R P) x x\<^sub>T"
+  unfolding and_leftp_def by (fastforce intro: crel_vs_intro elim: crel_vs_elim)
+term 0 (**)
+
+lemma map_transfer_inset:
+   "crel_vs ((and_leftp R0 (\<lambda>x. x\<in>set xs) ===>\<^sub>T R1) ===>\<^sub>T and_leftp (list_all2 R0) (op = xs) ===>\<^sub>T (list_all2 R1)) map map\<^sub>T"
+proof -
+  { fix f f\<^sub>T' xs\<^sub>T'
+    assume [transfer_rule]: "(and_leftp R0 (\<lambda>x. x\<in>set xs) ===>\<^sub>T R1) f f\<^sub>T'" and rx: "list_all2 R0 xs xs\<^sub>T'"
+    from rx[THEN and_leftp_leftset_intro] have "crel_vs (list_all2 R1) (map f xs) (map\<^sub>T' f\<^sub>T' xs\<^sub>T')"
+      apply (induction rule: list_all2_induct; unfold list.map map\<^sub>T'.simps)
+      subgoal premises [transfer_rule] by transfer_prover
+      subgoal premises [transfer_rule] by transfer_prover
+      done
+  }
+  hence [transfer_rule]: "((and_leftp R0 (\<lambda>x. x\<in>set xs) ===>\<^sub>T R1) ===> and_leftp (list_all2 R0) (op = xs) ===>\<^sub>T (list_all2 R1)) map map\<^sub>T'" 
+    by (fastforce elim: and_leftp_lefteq_elim)
+  show ?thesis
+    unfolding map\<^sub>T_def by transfer_prover
+qed
+
+lemma map_transfer_inset_unfolded:
+  fixes R0 R1 f f\<^sub>T' xs xs\<^sub>T
+  assumes "(and_leftp R0 (\<lambda>x. x\<in>set xs) ===>\<^sub>T R1) f f\<^sub>T'" "crel_vs (list_all2 R0) xs xs\<^sub>T"
+  shows "crel_vs (list_all2 R1) (map f xs) (map\<^sub>T . \<langle>f\<^sub>T'\<rangle> . xs\<^sub>T)"
+  apply (rule fun_app_lifted_transfer[THEN rel_funD, THEN rel_funD, where x=xs])
+   apply (rule fun_app_lifted_transfer[THEN rel_funD, THEN rel_funD, where x=f])
+    apply (fact map_transfer_inset)
+   apply (rule crel_vs_return)
+   apply (fact assms(1))
+  apply (rule and_leftp_crel_vs)
+  apply (rule and_leftp_lefteq_same)
+  apply (fact assms(2))
+  done
+
+lemma map_transfer_inset_unfolded':
+  fixes R0 R1 f f\<^sub>T' xs xs\<^sub>T
+  assumes "\<And>x x\<^sub>T'. R0 x x\<^sub>T' \<Longrightarrow> x\<in>set xs \<Longrightarrow> crel_vs R1 (f x) (f\<^sub>T' x\<^sub>T')" "crel_vs (list_all2 R0) xs xs\<^sub>T"
+  shows "crel_vs (list_all2 R1) (map f xs) (map\<^sub>T . \<langle>f\<^sub>T'\<rangle> . xs\<^sub>T)"
+  apply (rule map_transfer_inset_unfolded)
+   apply (rule rel_funI)
+   apply (rule assms(1))
+    apply (erule and_leftp_elim[where R=R0])
+    apply (assumption)
+   apply (erule and_leftp_elim[where R=R0])
+   apply (assumption)
+  apply (fact assms(2))
+  done
+
+lemma crel_vs_map_simple:
+  fixes R f f\<^sub>T' xs xs\<^sub>T
+  assumes "\<And>x. x \<in> set xs \<Longrightarrow> crel_vs op = (f x) (f\<^sub>T' x)" "crel_vs op = xs xs\<^sub>T"
+  shows "crel_vs op = (map f xs) (map\<^sub>T . \<langle>f\<^sub>T'\<rangle> . xs\<^sub>T)"
+  apply (rule map_transfer_inset_unfolded'[where ?R0.0="op =" and ?R1.0="op =", unfolded list.rel_eq])
+   apply clarify
+   apply (fact assms(1))
+  apply (fact assms(2))
+  done
+
+lemma map_transfer_inset0:
+  "crel_vs ((eq_onp (\<lambda>x. x\<in>set xs) ===>\<^sub>T R) ===>\<^sub>T eq_onp (op = xs) ===>\<^sub>T (list_all2 R)) map map\<^sub>T"
+  using map_transfer_inset[of "op =", unfolded list.rel_eq eq_onp_and_leftp_eq] .
+term 0 (**)
+
+lemma fold_transfer_inset:
+  fixes R0 R1 f f\<^sub>T' xs xs\<^sub>T
+  assumes "(and_leftp R0 (\<lambda>x. x\<in>set xs) ===>\<^sub>T R1 ===>\<^sub>T R1) f f\<^sub>T'" "crel_vs (list_all2 R0) xs xs\<^sub>T"
+  shows  "crel_vs (R1 ===>\<^sub>T R1) (fold f xs) (fold\<^sub>T . \<langle>f\<^sub>T'\<rangle> . xs\<^sub>T)"
+proof -
+  { fix f f\<^sub>T' xs\<^sub>T' a b
+    assume [transfer_rule]: "(and_leftp R0 (\<lambda>x. x\<in>set xs) ===>\<^sub>T R1 ===>\<^sub>T R1) f f\<^sub>T'" and rx: "list_all2 R0 xs xs\<^sub>T'"
+    from rx[THEN and_leftp_leftset_intro] have "crel_vs (R1 ===>\<^sub>T R1) (fold f xs) (fold\<^sub>T' f\<^sub>T' xs\<^sub>T')"
+      apply (induction rule: list_all2_induct; unfold fold.simps fold\<^sub>T'.simps)
+      subgoal premises [transfer_rule] by transfer_prover
+      subgoal premises [transfer_rule] by transfer_prover
+      done
+  }
+  hence [transfer_rule]: "((and_leftp R0 (\<lambda>x. x\<in>set xs) ===>\<^sub>T R1 ===>\<^sub>T R1) ===> and_leftp (list_all2 R0) (op = xs) ===>\<^sub>T R1 ===>\<^sub>T R1) fold fold\<^sub>T'" 
+    by (fastforce elim: and_leftp_lefteq_elim)
+  show ?thesis
+    unfolding fold\<^sub>T_def supply [transfer_rule] = assms(1) and_leftp_lefteq_same[THEN and_leftp_crel_vs, OF assms(2)] by transfer_prover    
+qed
+  
+end
+end
+
+definition K :: "'a \<Rightarrow> 'a \<Rightarrow> 'a \<Rightarrow> bool" where
+  "K x \<equiv> eq_onp (op = x)"
+
+lemma K_self: "K x x x"
+  unfolding K_def eq_onp_def by auto
+end
+ 
