scratch/dp/DP_Proof.thy
@@ -1,0 +1,14 @@
+theory DP_Proof
+  imports "./DP_CRelVS" "~~/src/HOL/Eisbach/Eisbach_Tools"
+begin           
+
+method dp_match uses induct simp simp\<^sub>T =
+  ( rule dp_consistency.consistentDP_intro,
+    rule induct,
+    unfold simp\<^sub>T;
+    rule dp_consistency.crel_vs_checkmem,
+    unfold simp,
+    ((match premises in _[transfer_rule]: _ (multi) \<Rightarrow> transfer_prover)
+      | (match conclusion in _ \<Rightarrow> transfer_prover)))
+
+end
